functional-programming-lean/src/monad-transformers/reader-io.md
@@ -70,6 +70,7 @@ Thus, `dirTree` is declared `partial`:
 ```lean
 {{#example_decl Examples/MonadTransformers.lean OldDirTree}}
 ```
+The call to `toEntry` is a [nested action](../hello-world/conveniences.md#nested-actions)—the parentheses are optional in positions where the arrow couldn't have any other meaning, such as `match`.
 When the filename doesn't correspond to an entry in the tree (e.g. because it is `..`), `dirTree` does nothing.
 When the filename is an ordinary file, `dirTree` calls a helper to show it with the current configuration.
 When the filename is a directory, it is shown with a helper, and then its contents are recursively shown in a new configuration in which the prefix has been extended to account for being in a new directory.
@@ -87,12 +88,76 @@ Similarly, `Config.inDirectory` extends the prefix with a directory marker:
 {{#example_decl Examples/MonadTransformers.lean inDirectory}}
 ```
 
-Iterating an IO action over a list of directory contents is achieved using `doList`:
+Iterating an IO action over a list of directory contents is achieved using `doList`.
+Like `mapM`, `doList` works for any monad:
 ```lean
 {{#example_decl Examples/MonadTransformers.lean doList}}
 ```
 
+
 ## Using a Custom Monad
+
+While this implementation of `doug` works, manually passing the configuration around is verbose and error-prone.
+The type system will not catch it if the wrong configuration is passed downwards, for instance.
+A reader effect ensures that the same configuration is passed to all recursive calls, unless it is manually overridden, and it helps make the code less verbose.
+
+To create a version of `IO` that is also a reader of `Config`, first define the type and its `Monad` instance, following the recipe from [the evaluator example](../monads/arithmetic.md#custom-environments).
+The difference between this `Monad` instance and the one for `Reader` is that this one uses `do`-notation in the `IO` monad as the body of the function, rather than applying `next` directly to the value returned from `result`.
+Any `IO` effects performed by `result` must occur before `next` is invoked, which is ensured by the `IO` monad's `bind` operator.
+
+The next step is to define a means of accessing the current configuration as part of `ConfigIO`:
+```lean
+{{#example_decl Examples/MonadTransformers.lean currentConfig}}
+```
+This is just like `read` from [the evaluator example](../monads/arithmetic.md#custom-environments), except it uses `IO`'s `pure` to return its value rather than doing so directly.
+Because entering a directory modifies the current configuration for the scope of a recursive call, it will be necessary to have a way to override a configuration:
+```lean
+{{#example_decl Examples/MonadTransformers.lean locally}}
+```
+
+Much of the code used in `doug` has no need for configurations, and `doug` calls ordinary Lean `IO` actions from the standard library that certainly don't need a `Config`.
+Ordinary `IO` actions can be run using `runIO`, which ignores the configuration argument:
+```lean
+{{#example_decl Examples/MonadTransformers.lean runIO}}
+```
+
+With these components, `showFileName` and `showDirName` can be updated to take their configuration arguments implicitly through the `ConfigIO` monad.
+They use [nested actions](../hello-world/conveniences.md#nested-actions) to retrieve the configuration, and `runIO` to actually execute the call to `IO.println`:
+```lean
+{{#example_decl Examples/MonadTransformers.lean MedShowFileDir}}
+```
+
+In the new version of `dirTree`, the calls to `toEntry` and `System.FilePath.readDir` are wrapped in `runIO`.
+Additionally, instead of building a new configuration and then requiring the programmer to keep track of which one to pass to recursive calls, it uses `locally` to naturally delimit the modified configuration to only a small region of the program, in which it is the _only_ valid configuration:
+```lean
+{{#example_decl Examples/MonadTransformers.lean MedDirTree}}
+```
+
+The new version of `main` only reverses the order of the arguments to `dirTree`:
+```lean
+{{#example_decl Examples/MonadTransformers.lean MedMain}}
+```
+
+This custom monad has a number of advantages over passing configurations manually:
+
+ 1. It is easier to ensure that configurations are passed down unchanged, except when changes are desired
+ 2. The concern of passing the configuration onwards is more clearly separated from the concern of printing directory contents
+ 3. As the program grows, there will be more and more intermediate layers that do nothing with configurations except propagate them, and these layers don't need to be rewritten as the configuration logic changes
+
+However, there are also some clear downsides:
+
+ 1. As the program evolves and the monad requires more features, each of the basic operators such as `locally` and `currentConfig` will need to be updated
+ 2. Wrapping ordinary `IO` actions in `runIO` is noisy and distracts from the flow of the program
+ 3. Writing monads by hand is repetitive, and the technique for adding a reader effect to another monad is a design pattern that requires documentation and communication
+
+Using a technique called _monad transformers_, all of these downsides can be addressed.
+A monad transformer takes a monad as an argument, and returns a new monad.
+Monad transformers consist of:
+ 1. A definition of the transformer itself, which is typically a function from types to types
+ 2. A `Monad` instance that assumes the inner type is already a monad
+ 3. An operator to "lift" an action from the inner monad to the transformed monad, akin to `runIO`
+
+## Adding a Reader to Any Monad
 
 
 
